spot/GC.SPOT.HeapExpansion.fst
@@ -1821,6 +1821,7 @@ let spot_chunked_cheney_promote_after_minor_promotion_head_preflight
            r.capacity_major_out r.capacity_fp_out r.capacity_fuel_out = true /\
          GenInv.chunked_chain_objects_blue
            r.capacity_major_out r.capacity_fp_out r.capacity_fuel_out /\
+         CheneyPreservation.chunked_fwd_targets_above_minor res.fwd_map /\
          (forall (x:U64.t).
            Seq.mem x (minor_reachable minor roots) /\
            minor_wosize minor x > 0 ==>
@@ -3540,6 +3541,7 @@ let spot_chunked_cheney_collect_after_minor_promotion_head_preflight
          U64.v collect.cmc_minor.bump == 0 /\
          collect.cmc_roots == rewrite_roots roots prom.fwd_map /\
          collect.cmc_fwd == prom.fwd_map /\
+         CheneyPreservation.chunked_fwd_targets_above_minor collect.cmc_fwd /\
          GenInv.chunked_major_alloc_shape
            collect.cmc_major collect.cmc_fp r.capacity_fuel_out /\
          SpecMajorAlloc.major_fl_chain_terminates
@@ -3578,9 +3580,7 @@ let spot_chunked_cheney_collect_after_minor_promotion_head_preflight
           U64.v (Obj.getTag hdr) < U64.v Obj.no_scan_tag /\
           j < U64.v (Obj.getWosize hdr) /\
           U64.v field_addr == U64.v src + j * U64.v mword /\
-          MH.read_word_in_major major field_addr == Some old /\
-          ChunkedUpdate.chunked_update_value_stable collect.cmc_fwd
-            (ChunkedUpdate.chunked_update_expected_value collect.cmc_fwd old) ==>
+          MH.read_word_in_major major field_addr == Some old ==>
           MH.read_word_in_major collect.cmc_major field_addr ==
             Some (ChunkedUpdate.chunked_update_expected_value
               collect.cmc_fwd old)) /\
@@ -3666,6 +3666,7 @@ let spot_chunked_cheney_gc_correct_after_preflight
          U64.v collect.cmc_minor.bump == 0 /\
          collect.cmc_roots == rewrite_roots roots prom.fwd_map /\
          collect.cmc_fwd == prom.fwd_map /\
+         CheneyPreservation.chunked_fwd_targets_above_minor collect.cmc_fwd /\
          GenInv.chunked_major_alloc_shape
            collect.cmc_major collect.cmc_fp r.capacity_fuel_out /\
          SpecMajorAlloc.major_fl_chain_terminates
@@ -3704,9 +3705,7 @@ let spot_chunked_cheney_gc_correct_after_preflight
           U64.v (Obj.getTag hdr) < U64.v Obj.no_scan_tag /\
           j < U64.v (Obj.getWosize hdr) /\
           U64.v field_addr == U64.v src + j * U64.v mword /\
-          MH.read_word_in_major major field_addr == Some old /\
-          ChunkedUpdate.chunked_update_value_stable collect.cmc_fwd
-            (ChunkedUpdate.chunked_update_expected_value collect.cmc_fwd old) ==>
+          MH.read_word_in_major major field_addr == Some old ==>
           MH.read_word_in_major collect.cmc_major field_addr ==
             Some (ChunkedUpdate.chunked_update_expected_value
               collect.cmc_fwd old)) /\
